Refine cheats in pan_to_wordProof

pancake/pan_to_wordScript.sml
@@ -9,7 +9,7 @@ open preamble
 val _ = new_theory "pan_to_word";
 
 
-Definition compile_prog:
+Definition compile_prog_def:
   compile_prog prog =
   let prog = pan_to_crep$compile_prog prog;
       prog = crep_to_loop$compile_prog prog in
