pancake/proofs/pan_to_wordProofScript.sml
@@ -29,48 +29,47 @@ Definition mk_mem_def:
 End
 
 Definition loop_state_def:
-  loop_state (s:('a,'ffi) crepSem$state) crep_code =
+  loop_state (s:('a,'ffi) crepSem$state) crep_code ck =
   let ctxt = mk_ctxt FEMPTY (make_funcs crep_code) 0 (get_eids crep_code) in
   <| locals   := LN;
      globals  := FEMPTY;
      memory   := mk_mem ctxt s.memory;
      mdomain := s.memaddrs;
      code     := fromAList (crep_to_loop$compile_prog crep_code);
-     clock    := ARB;
+     clock    := ck;
      be       := s.be;
      ffi      := s.ffi|>
 End
 
+
 Theorem get_eids_equivs:
-   !pan_code. equivs (FRANGE ((get_eids pan_code):mlstring |-> 'a word))
-          ((get_eids (compile_prog pan_code)): 'a word set)
+   !prog. equivs (FRANGE ((get_eids prog):mlstring |-> 'a word))
+          ((get_eids (compile_prog prog)): 'a word set)
 Proof
-  cheat
-
-QED
-
-Theorem all_distinct_first_compile_prog:
-  ALL_DISTINCT (MAP FST pan_code) ==>
-  ALL_DISTINCT (MAP FST (pan_to_crep$compile_prog pan_code))
-Proof
-  cheat
-QED
-
-Theorem alookup_compile_prog_code:
-  ALOOKUP pan_code start = SOME ([],prog) ==>
-  ALOOKUP (pan_to_crep$compile_prog pan_code) start =
-  SOME ([],
-        comp_func (make_funcs pan_code) (get_eids pan_code) [] prog)
-Proof
+  rw [] >>
+  fs [equivs_def] >>
+  rw [] >>
+  fs [EQ_IMP_THM] >>
+  conj_tac
+  >- (
+   rw [] >>
+   fs [pan_to_crepTheory.compile_prog_def] >>
+   fs [crep_to_loopTheory.get_eids_def] >>
+   fs [MAP_MAP_o] >>
+   cheat) >>
   cheat
 QED
 
 
 Theorem state_rel_imp_semantics:
-  s.memaddrs = t.mdomain ∧
-  s.be = t.be ∧
-  s.ffi = t.ffi ∧
+  t.memory = mk_mem
+             (mk_ctxt FEMPTY (make_funcs (compile_prog pan_code)) 0
+              (get_eids (compile_prog pan_code))) s.memory /\
+  t.mdomain = s.memaddrs ∧
+  t.be = s.be ∧
+  t.ffi = s.ffi ∧
   ALL_DISTINCT (MAP FST pan_code) ∧
+  ALOOKUP pan_code start = SOME ([],prog) ∧
   s.code = alist_to_fmap pan_code ∧
   t.code = fromAList (pan_to_word$compile_prog pan_code) ∧
   s.locals = FEMPTY ∧ size_of_eids pan_code < dimword (:α) ∧
@@ -78,7 +77,8 @@ Theorem state_rel_imp_semantics:
   (∀ad f.
    s.memory ad = Label f ⇒
    ∃n m. FLOOKUP (make_funcs (compile_prog pan_code)) f = SOME (n,m)) /\
-  ALOOKUP pan_code start = SOME ([],prog) ∧
+   FLOOKUP (make_funcs (compile_prog pan_code)) start = SOME (lc,0) /\
+  lookup 0 t.locals = SOME (Loc 1 0) /\
   semantics s start <> Fail ==>
   semantics (t:('a,'b, 'ffi) wordSem$state) lc =
   semantics (s:('a,'ffi) panSem$state) start
@@ -86,7 +86,7 @@ Proof
   rw [] >>
   ‘state_rel s (crep_state s pan_code)’ by (
     fs [pan_to_crepProofTheory.state_rel_def, crep_state_def]) >>
-  drule pan_to_crepProofTheory.state_rel_imp_semantics >>
+  drule (GEN_ALL pan_to_crepProofTheory.state_rel_imp_semantics) >>
   disch_then (qspecl_then [‘start’, ‘prog’ , ‘pan_code’] mp_tac) >>
   fs [] >>
   impl_tac
@@ -95,9 +95,9 @@ Proof
   pop_assum (assume_tac o GSYM) >>
   fs [] >>
   ‘(crep_state s pan_code).memaddrs =
-   (loop_state (crep_state s pan_code) (pan_to_crep$compile_prog pan_code)).mdomain’ by
+   (loop_state (crep_state s pan_code) (pan_to_crep$compile_prog pan_code) t.clock).mdomain’ by
     fs [crep_state_def, loop_state_def] >>
-  drule crep_to_loopProofTheory.state_rel_imp_semantics >>
+  drule (GEN_ALL crep_to_loopProofTheory.state_rel_imp_semantics) >>
   disch_then (qspecl_then [‘start’, ‘comp_func (make_funcs pan_code) (get_eids pan_code) [] prog’,
                            ‘lc’, ‘compile_prog pan_code’] mp_tac) >>
   impl_tac
@@ -110,14 +110,83 @@ Proof
    conj_tac
    >- fs [get_eids_equivs] >>
    conj_tac >- fs [crep_to_loopProofTheory.globals_rel_def] >>
-   conj_tac >- metis_tac [all_distinct_first_compile_prog] >>
-   conj_tac >- metis_tac [alookup_compile_prog_code] >>
-   cheat) >>
+   conj_tac >- metis_tac [first_compile_prog_all_distinct] >>
+   metis_tac [alookup_compile_prog_code]) >>
   strip_tac >>
   pop_assum (assume_tac o GSYM) >>
   fs [] >>
   pop_assum kall_tac >>
-  match_mp_tac fstate_rel_imp_semantics >>
-  cheat
+  match_mp_tac (GEN_ALL fstate_rel_imp_semantics) >>
+  MAP_EVERY qexists_tac [‘ARB’, ‘compile_prog (compile_prog pan_code)’] >>
+  fs [] >>
+  conj_tac
+  >- (
+   fs [st_rel_def] >>
+   conj_tac
+   >- (
+    fs [loop_removeProofTheory.state_rel_def] >>
+    qexists_tac ‘fromAList (comp_prog (compile_prog (compile_prog pan_code)))’ >>
+    fs [] >>
+    rpt gen_tac >>
+    strip_tac >>
+    fs [loop_state_def, crep_state_def] >>
+    cheat) >>
+   fs [loop_to_wordProofTheory.state_rel_def] >>
+   fs [loop_state_def, crep_state_def] >>
+   fs [globals_rel_def] >>
+   fs [] >>
+   fs [loop_to_wordProofTheory.code_rel_def] >>
+   rpt gen_tac >>
+   strip_tac >>
+   conj_tac
+   >- (
+    fs [pan_to_wordTheory.compile_prog_def,
+        loop_to_wordTheory.compile_def] >>
+    fs [loop_to_wordTheory.compile_prog_def] >>
+    fs [lookup_fromAList] >>
+    drule ALOOKUP_MEM >>
+    strip_tac >>
+    match_mp_tac wordPropsTheory.ALL_DISTINCT_MEM_IMP_ALOOKUP_SOME >>
+    reverse conj_tac
+    >- (
+     fs [MEM_MAP] >>
+     qexists_tac ‘(name,params,body)’ >>
+     fs []) >>
+    cheat) >>
+   conj_tac
+   >- cheat >>
+   cheat) >>
+  fs [loop_state_def, crep_state_def] >>
+  fs [pan_to_wordTheory.compile_prog_def] >>
+  qpat_x_assum ‘FLOOKUP _ _ = SOME (lc,0)’ assume_tac >>
+  fs [crep_to_loopProofTheory.make_funcs_def] >>
+
+
+
+
+     )
+
+
+    )
+
+
+
+
+
+   >- (
+    conj_tac
+    >- (
+     fs [mk_mem_def] >>
+     fs [FUN_EQ_THM] >>
+     rw [] >>
+     cases_on ‘s.memory ad’ >>
+     fs [wlab_wloc_def]
+
+
+   )
+
+
+
+
 QED
 val _ = export_theory();
